Rocq/src/Spec.v
@@ -6,6 +6,7 @@ From Verilog Require Import Utils.
 
 Import ListNotations.
 Import Nat.
+
 Import Expr.
 Import Path.
 Import Utils.
@@ -15,158 +16,165 @@ Set Implicit Arguments.
 Module Spec.
 
   Section SpecDef.
-    Fixpoint pass1 e :=
+    Fixpoint determine e :=
       match e with
       | EAtom op => op
-      | EBinOp lhs rhs => max (pass1 lhs) (pass1 rhs)
-      | EUnOp arg => pass1 arg
-      | ECast arg => pass1 arg
+      | EBinOp lhs rhs => max (determine lhs) (determine rhs)
+      | EUnOp arg => determine arg
+      | ECast arg => determine arg
       | EComp _ _ => 1
       | ELogic _ _ => 1
       | EReduction _ => 1
-      | EShift lhs _ => pass1 lhs
+      | EShift lhs _ => determine lhs
       | EAssign lval _ => lval
       | EShiftAssign lval _ => lval
-      | ECond _ lhs rhs => max (pass1 lhs) (pass1 rhs)
-      | EConcat args => sum (map pass1 args)
-      | ERepl i arg => i * pass1 arg
+      | ECond _ lhs rhs => max (determine lhs) (determine rhs)
+      | EConcat args => sum (map determine args)
+      | ERepl i arg => i * determine arg
       end
     .
 
-    Variable pass2 : Expr -> path -> nat.
+    Variable propagate : Expr -> path -> nat.
 
-    Definition binop_pass2 :=
-      forall e p lhs rhs,
+    Definition binop_propagate := forall e p lhs rhs,
         e @[p] = Some (EBinOp lhs rhs) ->
-        pass2 e (p ++ [Lhs]) = pass2 e p /\ pass2 e (p ++ [Rhs]) = pass2 e p.
+        propagate e (p ++ [Left]) = propagate e p /\
+          propagate e (p ++ [Right]) = propagate e p.
 
-    Definition unop_pass2 :=
-      forall e p arg, e @[p] = Some (EUnOp arg) -> pass2 e (p ++ [Arg]) = pass2 e p.
+    Definition unop_propagate := forall e p arg,
+        e @[p] = Some (EUnOp arg) ->
+        propagate e (p ++ [Arg]) = propagate e p.
 
-    Definition cast_pass2 :=
-      forall e p arg, e @[p] = Some (ECast arg) -> pass2 e (p ++ [Arg]) = pass1 arg.
+    Definition cast_propagate := forall e p arg,
+        e @[p] = Some (ECast arg) ->
+        propagate e (p ++ [Arg]) = determine arg.
 
-    Definition comp_pass2 :=
-      forall e p lhs rhs,
+    Definition comp_propagate := forall e p lhs rhs,
         e @[p] = Some (EComp lhs rhs) ->
-        forall s, s = max (pass1 lhs) (pass1 rhs) ->
-             pass2 e (p ++ [Lhs]) = s /\ pass2 e (p ++ [Rhs]) = s.
+        forall s, s = max (determine lhs) (determine rhs) ->
+             propagate e (p ++ [Left]) = s /\
+               propagate e (p ++ [Right]) = s.
 
-    Definition logic_pass2 :=
-      forall e p lhs rhs,
-        e @[p] = Some (ELogic lhs rhs) -> pass2 e (p ++ [Lhs]) = pass1 lhs /\ pass2 e (p ++ [Rhs]) = pass1 rhs.
+    Definition logic_propagate := forall e p lhs rhs,
+        e @[p] = Some (ELogic lhs rhs) ->
+        propagate e (p ++ [Left]) = determine lhs /\
+          propagate e (p ++ [Right]) = determine rhs.
 
-    Definition red_pass2 :=
-      forall e p arg, e @[p] = Some (EReduction arg) -> pass2 e (p ++ [Arg]) = pass1 arg.
+    Definition red_propagate := forall e p arg,
+        e @[p] = Some (EReduction arg) ->
+        propagate e (p ++ [Arg]) = determine arg.
 
-    Definition shift_pass2 :=
-      forall e p lhs rhs, e @[p] = Some (EShift lhs rhs) ->
-                     pass2 e (p ++ [Lhs]) = pass2 e p /\ pass2 e (p ++ [Rhs]) = pass1 rhs.
+    Definition shift_propagate := forall e p lhs rhs,
+        e @[p] = Some (EShift lhs rhs) ->
+        propagate e (p ++ [Left]) = propagate e p /\
+          propagate e (p ++ [Right]) = determine rhs.
 
-    Definition assign_pass2 :=
-      forall e p lval arg,
+    Definition assign_propagate := forall e p lval arg,
         e @[p] = Some (EAssign lval arg) ->
-        forall s, s = max (pass1 arg) lval -> pass2 e (p ++ [Arg]) = s.
+        forall s, s = max (determine arg) lval ->
+             propagate e (p ++ [Arg]) = s.
 
-    Definition shiftassign_pass2 :=
-      forall e p lval arg, e @[p] = Some (EShiftAssign lval arg) -> pass2 e (p ++ [Arg]) = pass1 arg.
+    Definition shiftassign_propagate := forall e p lval arg,
+        e @[p] = Some (EShiftAssign lval arg) ->
+        propagate e (p ++ [Arg]) = determine arg.
 
-    Definition cond_pass2 :=
-      forall e p cond lhs rhs,
+    Definition cond_propagate := forall e p cond lhs rhs,
         e @[p] = Some (ECond cond lhs rhs) ->
-        pass2 e (p ++ [Lhs]) = pass2 e p /\ pass2 e (p ++ [Rhs]) = pass2 e p /\
-          pass2 e (p ++ [Cond]) = pass1 cond.
+        propagate e (p ++ [Left]) = propagate e p /\
+          propagate e (p ++ [Right]) = propagate e p /\
+          propagate e (p ++ [Arg]) = determine cond.
 
-    Definition concat_pass2 :=
-      forall e p args, e @[p] = Some (EConcat args) ->
-                  forall i f, nth_error args i = Some f -> pass2 e (p ++ [Args i]) = pass1 f.
+    Definition concat_propagate := forall e p args,
+        e @[p] = Some (EConcat args) ->
+        forall i f, nth_error args i = Some f ->
+               propagate e (p ++ [Args i]) = determine f.
 
-    Definition repl_pass2 :=
-      forall e p i arg, e @[p] = Some (ERepl i arg) -> pass2 e (p ++ [Arg]) = pass1 arg.
+    Definition repl_propagate := forall e p i arg,
+        e @[p] = Some (ERepl i arg) ->
+        propagate e (p ++ [Arg]) = determine arg.
 
-    Definition toplevel_pass2 := forall e, pass2 e [] = pass1 e.
+    Definition toplevel_propagate := forall e, propagate e [] = determine e.
 
-    Definition pass2_def :=
-      toplevel_pass2 /\ binop_pass2 /\ unop_pass2 /\ cast_pass2 /\
-        comp_pass2 /\ logic_pass2 /\ red_pass2 /\ shift_pass2 /\
-        assign_pass2 /\ shiftassign_pass2 /\ cond_pass2 /\
-        concat_pass2 /\ repl_pass2.
+    Definition propagate_def :=
+      toplevel_propagate /\ binop_propagate /\ unop_propagate /\ cast_propagate /\
+        comp_propagate /\ logic_propagate /\ red_propagate /\ shift_propagate /\
+        assign_propagate /\ shiftassign_propagate /\ cond_propagate /\
+        concat_propagate /\ repl_propagate.
   End SpecDef.
 
-  Theorem pass2_val : forall p e, IsPath e p -> forall f, pass2_def f -> exists n, f e p = n.
+  Theorem propagate_val : forall f, propagate_def f -> forall p e, IsPath e p -> exists n, f e p = n.
   Proof.
     induction p using path_ind; intros.
     - firstorder.
     - assert (He: IsPath e p /\ exists f, e @[p] = Some f /\ IsPath f [x]).
-      + split. apply (IsPath_prefix _ _ H). apply IsPath_chunk. assumption.
+      + split. apply (IsPath_prefix _ _ H0). apply IsPath_chunk. assumption.
       + destruct He as [H1 [expr [H2 H3]]].
-        destruct expr; inv H3; destruct (IHp _ H1 _ H0); try (eexists; firstorder).
+        destruct expr; inv H3; destruct (IHp _ H1); try (eexists; firstorder).
   Qed.
 
-  Ltac pass2_def_split :=
+  Ltac propagate_def_split :=
     match goal with
-    | [ H: pass2_def _ |- _ ] =>
+    | [ H: propagate_def _ |- _ ] =>
         destruct H as [?HTopLevel [?HBinOp [?HUnOp [?HCast [?HComp [?HLogic [?HRed [?HShift [?HAssign [?HShiftAssign [?HCond [?HConcat ?HRepl]]]]]]]]]]]]
     end
   .
 
-  Theorem pass2_unique : forall p e,
-      IsPath e p -> forall f1 f2, pass2_def f1 -> pass2_def f2 -> f1 e p = f2 e p.
+  Theorem propagate_unique : forall p e,
+      IsPath e p -> forall f1 f2, propagate_def f1 -> propagate_def f2 -> f1 e p = f2 e p.
   Proof.
-    Ltac _pass2_unique_tac :=
+    Ltac _propagate_unique_tac :=
       match goal with
-      | [ G: _ _ _ = _ _ _, F: _ @[_] = Some (EBinOp _ _), H: binop_pass2 _ |- _ ] =>
+      | [ G: _ _ _ = _ _ _, F: _ @[_] = Some (EBinOp _ _), H: binop_propagate _ |- _ ] =>
           destruct (H _ _ _ _ F); rewrite G in *; assumption
-      | [ G: _ _ _ = _ _ _, F: _ @[_] = Some (EUnOp _), H: unop_pass2 _ |- _ ] =>
+      | [ G: _ _ _ = _ _ _, F: _ @[_] = Some (EUnOp _), H: unop_propagate _ |- _ ] =>
           apply H in F; rewrite G in *; assumption
-      | [ F: _ @[_] = Some (ELogic _ _), H: logic_pass2 _ |- _ ] =>
+      | [ F: _ @[_] = Some (ELogic _ _), H: logic_propagate _ |- _ ] =>
           destruct (H _ _ _ _ F); assumption
-      | [ F: _ @[_] = Some (EReduction _), H: red_pass2 _ |- _ ] =>
+      | [ F: _ @[_] = Some (EReduction _), H: red_propagate _ |- _ ] =>
           apply H in F; assumption
-      | [ G: _ _ _ = _ _ _, F: _ @[_] = Some (EShift _ _), H: shift_pass2 _ |- _ ] =>
+      | [ G: _ _ _ = _ _ _, F: _ @[_] = Some (EShift _ _), H: shift_propagate _ |- _ ] =>
           destruct (H _ _ _ _ F); assumption || rewrite G in *; assumption
-      | [ F: _ @[_] = Some (EAssign _ _), H: assign_pass2 _ |- _ ] =>
+      | [ F: _ @[_] = Some (EAssign _ _), H: assign_propagate _ |- _ ] =>
           apply (H _ _ _ _ F); reflexivity
-      | [ F: _ @[_] = Some (EShiftAssign _ _), H: shiftassign_pass2 _ |- _ ] =>
+      | [ F: _ @[_] = Some (EShiftAssign _ _), H: shiftassign_propagate _ |- _ ] =>
           apply (H _ _ _ _ F)
-      | [ G: _ _ _ = _ _ _, F: _ @[_] = Some (ECond _ _ _), H: cond_pass2 _ |- _ ] =>
+      | [ G: _ _ _ = _ _ _, F: _ @[_] = Some (ECond _ _ _), H: cond_propagate _ |- _ ] =>
           destruct (H _ _ _ _ _ F) as [? []]; assumption || rewrite G in *; assumption
-      | [ G: nth_error _ _ = _, F: _ @[_] = Some (EConcat _), H: concat_pass2 _ |- _ ] =>
-          apply (H _ _ _ F _ _ G)
-      | [ F: _ @[_] = Some (ERepl _ _), H: repl_pass2 _ |- _ ] =>
+      | [ G: nth_error _ _ = _, F: _ @[_] = Some (EConcat _),
+              H: concat_propagate _ |- _ ] => apply (H _ _ _ F _ _ G)
+      | [ F: _ @[_] = Some (ERepl _ _), H: repl_propagate _ |- _ ] =>
           apply (H _ _ _ _ F)
       end
     .
     assert (Heq: forall x y m : nat, x = m -> y = m -> x = y). { intros. subst. reflexivity. }
     induction p using path_ind; intros.
-    - apply eq_trans with (y := pass1 e). firstorder. symmetry. firstorder.
+    - apply eq_trans with (y := determine e). firstorder. symmetry. firstorder.
     - assert (He: IsPath e p /\ exists f, e @[p] = Some f /\ IsPath f [x]).
       + split. apply (IsPath_prefix _ _ H). apply IsPath_chunk. assumption.
       + destruct He as [H2 [expr [H3 H4]]].
         assert (Hf: f1 e p = f2 e p). apply (IHp _ H2 _ _ H0 H1). clear IHp.
-        destruct expr; inv H4; repeat pass2_def_split.
-        * apply Heq with (m := f1 e p); _pass2_unique_tac.
-        * apply Heq with (m := f1 e p); _pass2_unique_tac.
-        * apply Heq with (m := f1 e p); _pass2_unique_tac.
-        * apply Heq with (m := pass1 expr); firstorder.
-        * apply Heq with (m := max (pass1 expr1) (pass1 expr2)).
-          destruct (HComp0 _ _ _ _ H3 (max (pass1 expr1) (pass1 expr2))); auto.
-          destruct (HComp _ _ _ _ H3 (max (pass1 expr1) (pass1 expr2))); auto.
-        * apply eq_trans with (y := max (pass1 expr1) (pass1 expr2)).
-          destruct (HComp0 _ _ _ _ H3 (max (pass1 expr1) (pass1 expr2))); auto.
-          destruct (HComp _ _ _ _ H3 (max (pass1 expr1) (pass1 expr2))); auto.
-        * apply Heq with (m := pass1 expr1); _pass2_unique_tac.
-        * apply Heq with (m := pass1 expr2); _pass2_unique_tac.
-        * apply Heq with (m := pass1 expr); _pass2_unique_tac.
-        * apply Heq with (m := f1 e p); _pass2_unique_tac.
-        * apply Heq with (m := pass1 expr2); _pass2_unique_tac.
-        * apply Heq with (m := max (pass1 expr) lval); _pass2_unique_tac.
-        * apply Heq with (m := pass1 expr); _pass2_unique_tac.
-        * apply Heq with (m := pass1 expr1); _pass2_unique_tac.
-        * apply Heq with (m := f1 e p); _pass2_unique_tac.
-        * apply Heq with (m := f1 e p); _pass2_unique_tac.
-        * apply Heq with (m := pass1 e0); _pass2_unique_tac.
-        * apply Heq with (m := pass1 expr); _pass2_unique_tac.
+        destruct expr; inv H4; repeat propagate_def_split.
+        * apply Heq with (m := f1 e p); _propagate_unique_tac.
+        * apply Heq with (m := f1 e p); _propagate_unique_tac.
+        * apply Heq with (m := f1 e p); _propagate_unique_tac.
+        * apply Heq with (m := determine expr); firstorder.
+        * apply Heq with (m := max (determine expr1) (determine expr2)).
+          destruct (HComp0 _ _ _ _ H3 (max (determine expr1) (determine expr2))); auto.
+          destruct (HComp _ _ _ _ H3 (max (determine expr1) (determine expr2))); auto.
+        * apply eq_trans with (y := max (determine expr1) (determine expr2)).
+          destruct (HComp0 _ _ _ _ H3 (max (determine expr1) (determine expr2))); auto.
+          destruct (HComp _ _ _ _ H3 (max (determine expr1) (determine expr2))); auto.
+        * apply Heq with (m := determine expr1); _propagate_unique_tac.
+        * apply Heq with (m := determine expr2); _propagate_unique_tac.
+        * apply Heq with (m := determine expr); _propagate_unique_tac.
+        * apply Heq with (m := f1 e p); _propagate_unique_tac.
+        * apply Heq with (m := determine expr2); _propagate_unique_tac.
+        * apply Heq with (m := max (determine expr) lval); _propagate_unique_tac.
+        * apply Heq with (m := determine expr); _propagate_unique_tac.
+        * apply Heq with (m := determine expr1); _propagate_unique_tac.
+        * apply Heq with (m := f1 e p); _propagate_unique_tac.
+        * apply Heq with (m := f1 e p); _propagate_unique_tac.
+        * apply Heq with (m := determine e0); _propagate_unique_tac.
+        * apply Heq with (m := determine expr); _propagate_unique_tac.
   Qed.
-
 End Spec.
