Rocq/src/Equiv.v
@@ -1,0 +1,222 @@
+From Stdlib Require Import Lists.List.
+From Stdlib Require Import PeanoNat.
+
+From Verilog Require Import Expr.
+From Verilog Require Import Path.
+From Verilog Require Import Spec.
+From Verilog Require Import TypeSystem.
+From Verilog Require Import Utils.
+
+Import ListNotations.
+Import Nat.
+
+Import Expr.
+Import Path.
+Import Spec.
+Import TypeSystem.
+Import Utils.
+
+Set Implicit Arguments.
+
+Module Equiv.
+  Lemma synth_check_determine_order : forall e1 e2 t1 t2 f1 f2,
+      e1 ==> t1 -| f1 -> e2 <== t2 -| f2 -> t2 <= t1 -> determine e2 <= determine e1.
+  Proof.
+    intros. destruct (synth_must_be_determine H). subst. destruct (synth_determine e2).
+    apply (synth_check_order H2) in H0. apply (le_trans _ _ _ H0 H1).
+  Qed.
+
+  Theorem spec_implies_ts : forall f1,
+      propagate_def f1 -> forall e f2, e ==> (determine e) -| f2 ->
+                                 forall p, IsPath e p -> forall n, f1 e p = n -> f2 p = Some n.
+  Proof.
+    Ltac _gen_eq_spec_ts :=
+      match goal with
+      | [ F: _ @[_] = Some (EBinOp _ _), H: binop_propagate _ |- _ ] =>
+          destruct (H _ _ _ _ F)
+      | [ F: _ @[_] = Some (EUnOp _), H: unop_propagate _ |- _ ] =>
+          apply H in F
+      | [ F: _ @[_] = Some (ECast _), H: cast_propagate _ |- _ ] =>
+          apply H in F
+      | [ F: _ @[_] = Some (EComp _ _), H: comp_propagate _ |- _ ] =>
+          destruct (H _ _ _ _ F _ (eq_refl _))
+      | [ F: _ @[_] = Some (ELogic _ _), H: logic_propagate _ |- _ ] =>
+          destruct (H _ _ _ _ F)
+      | [ F: _ @[_] = Some (EReduction _), H: red_propagate _ |- _ ] =>
+          apply H in F
+      | [ F: _ @[_] = Some (EShift _ _), H: shift_propagate _ |- _ ] =>
+          destruct (H _ _ _ _ F)
+      | [ F: _ @[_] = Some (EAssign _ _), H: assign_propagate _ |- _ ] =>
+          apply H in F
+      | [ F: _ @[_] = Some (EShiftAssign _ _), H: shiftassign_propagate _ |- _ ] =>
+          apply H in F
+      | [ F: _ @[_] = Some (ECond _ _ _), H: cond_propagate _ |- _ ] =>
+          destruct (H _ _ _ _ _ F) as [? [? ?]]
+      | [ G: nth_error _ _ = _, F: _ @[_] = Some (EConcat _),
+              H: concat_propagate _ |- _ ] =>
+          specialize (H _ _ _ F _ _ G)
+      | [ F: _ @[_] = Some (ERepl _ _), H: repl_propagate _ |- _ ] =>
+          specialize (H _ _ _ _ F)
+      end
+    .
+    Ltac _tac_spec_ts :=
+      match goal with
+      | [ H: ?x = ?n, G: _ <== ?n -| ?f |- ?f _ = Some ?x ] =>
+          rewrite H; apply (check_root G)
+      | [ H: ?x = ?n, G: _ ==> ?n -| ?f |- ?f _ = Some ?x ] =>
+          rewrite H; apply (synth_root G)
+      | [ H: ?x ==> _ -| ?f |- ?f [] = Some (determine ?x) ] =>
+          destruct (synth_must_be_determine H); assumption
+      end
+    .
+    induction p using path_ind; intros; propagate_def_split.
+    - rewrite (synth_root H0). unfold toplevel_propagate in HTopLevel.
+      rewrite HTopLevel in H2. subst. reflexivity.
+    - apply IsPath_chunk in H1. destruct H1 as [e' [He Hf]].
+      destruct (synth_sub_expr _ H0 He) as [t' [f' [[H3|H3] H4]]];
+        rewrite H4; specialize (IHp (sub_expr_valid _ _ He) (f1 e p) (eq_refl _));
+        specialize (H4 []); rewrite app_nil_r in H4; simpl in H4; rewrite H4 in IHp;
+        destruct e'.
+      + inv Hf.
+      + _gen_eq_spec_ts; inv Hf; inv H3; inv IHp; simpl; _tac_spec_ts.
+      + _gen_eq_spec_ts; inv Hf; inv H3; inv IHp; simpl; _tac_spec_ts.
+      + _gen_eq_spec_ts. inv Hf; inv H3. simpl. rewrite He; simpl; _tac_spec_ts.
+      + _gen_eq_spec_ts; inv Hf; inv H3.
+        * rewrite (max_l _ _ (synth_check_determine_order H7 H10 (le_refl _))) in *.
+          rewrite H; simpl; _tac_spec_ts.
+        * rewrite (max_r _ _ (synth_check_determine_order H10 H7 (le_refl _))) in *.
+          rewrite H. destruct (synth_must_be_determine H10). simpl. rewrite <- H2.
+          apply (check_root H7).
+        * rewrite (max_l _ _ (synth_check_determine_order H7 H10 (le_refl _))) in *.
+          rewrite H1. destruct (synth_must_be_determine H7). simpl. rewrite <- H2.
+          apply (check_root H10).
+        * rewrite (max_r _ _ (synth_check_determine_order H10 H7 (le_refl _))) in *.
+          rewrite H1; simpl; _tac_spec_ts.
+      + _gen_eq_spec_ts; inv Hf; inv H3.
+        * rewrite H; simpl; _tac_spec_ts.
+        * rewrite H1; simpl; _tac_spec_ts.
+      + _gen_eq_spec_ts; inv Hf; inv H3. rewrite He; simpl; _tac_spec_ts.
+      + _gen_eq_spec_ts; inv Hf; inv H3; inv IHp; simpl; try _tac_spec_ts.
+        rewrite H1; simpl; _tac_spec_ts.
+      + _gen_eq_spec_ts; inv Hf; inv H3; simpl; specialize (He _ (eq_refl _));
+        rewrite He.
+        * destruct (synth_determine e'). rewrite (max_r _ _ (synth_check_order H H7)).
+          apply (check_root H7).
+        * destruct (synth_must_be_determine H5). subst.
+          rewrite (max_l _ _ (lt_le_incl _ _ H8)). assumption.
+      + _gen_eq_spec_ts; inv Hf; inv H3; inv IHp; simpl. rewrite He; simpl; _tac_spec_ts.
+      + _gen_eq_spec_ts; inv Hf; inv H3; inv IHp; simpl; try _tac_spec_ts.
+        * rewrite H5; simpl; _tac_spec_ts.
+        * rewrite H5; simpl; _tac_spec_ts.
+      + inv Hf. _gen_eq_spec_ts. inv H3. repeat gen_nth. rewrite HConcat. simpl.
+        rewrite H. specialize (H5 _ _ _ _ H6 H2 H); simpl; _tac_spec_ts.
+      + _gen_eq_spec_ts; inv Hf; inv H3. simpl. rewrite HRepl; simpl; _tac_spec_ts.
+      + inv Hf.
+      + _gen_eq_spec_ts; inv Hf; inv H3; try (inv H2); inv IHp; simpl; _tac_spec_ts.
+      + _gen_eq_spec_ts; inv Hf; inv H3; try (inv H); inv IHp; simpl; _tac_spec_ts.
+      + _gen_eq_spec_ts; inv Hf; inv H3; inv H1; simpl; rewrite He; simpl; _tac_spec_ts.
+      + destruct (HComp _ _ _ _ He _ (eq_refl _)); inv Hf; inv H3; inv H5.
+        * rewrite (max_l _ _ (synth_check_determine_order H9 H12 (le_refl _))) in *.
+          rewrite H; simpl; _tac_spec_ts.
+        * rewrite (max_r _ _ (synth_check_determine_order H12 H9 (le_refl _))) in *.
+          rewrite H. destruct (synth_must_be_determine H12). simpl. rewrite <- H3.
+          apply (check_root H9).
+        * rewrite (max_l _ _ (synth_check_determine_order H9 H12 (le_refl _))) in *.
+          rewrite H1. destruct (synth_must_be_determine H9). simpl. rewrite <- H3.
+          apply (check_root H12).
+        * rewrite (max_r _ _ (synth_check_determine_order H12 H9 (le_refl _))) in *.
+          rewrite H1; simpl; _tac_spec_ts.
+      + _gen_eq_spec_ts; inv Hf; inv H3; inv H5.
+        * rewrite H; simpl; _tac_spec_ts.
+        * rewrite H1; simpl; _tac_spec_ts.
+      + _gen_eq_spec_ts; inv Hf; inv H3; inv H1; rewrite He; simpl; _tac_spec_ts.
+      + _gen_eq_spec_ts; inv Hf; inv H3; try (inv H2); inv IHp; simpl; try _tac_spec_ts.
+        rewrite H1. simpl; _tac_spec_ts.
+      + _gen_eq_spec_ts; inv Hf; inv H3; inv H2; simpl; specialize (He _ (eq_refl _));
+        rewrite He.
+        * destruct (synth_determine e'). rewrite (max_r _ _ (synth_check_order H2 H9)).
+          apply (check_root H9).
+        * destruct (synth_must_be_determine H7). subst.
+          rewrite (max_l _ _ (lt_le_incl _ _ H10)). assumption.
+      + _gen_eq_spec_ts; inv Hf; inv H3; inv H2; inv IHp; simpl;
+        rewrite He; _tac_spec_ts.
+      + _gen_eq_spec_ts; inv Hf; inv H3; try (inv H2); inv IHp; simpl; try _tac_spec_ts.
+        rewrite H5; _tac_spec_ts.
+      + inv Hf. _gen_eq_spec_ts. inv H3. inv H1; repeat gen_nth. rewrite HConcat. simpl.
+        rewrite H1. specialize (H9 _ _ _ _ H6 H3 H1); _tac_spec_ts.
+      + _gen_eq_spec_ts; inv Hf; inv H3; inv H2; simpl. rewrite HRepl; _tac_spec_ts.
+  Qed.
+
+  Theorem ts_implies_spec : forall f1,
+      propagate_def f1 -> forall e f2, e ==> (determine e) -| f2 ->
+                                 forall p, IsPath e p -> forall n, f2 p = Some n -> f1 e p = n.
+  Proof.
+    induction p using path_ind; intros; propagate_def_split.
+    - destruct (synth_must_be_determine H0). rewrite H3 in H2. inv H2. apply HTopLevel.
+    - apply IsPath_chunk in H1. destruct H1 as [e' [He Hf]].
+      specialize (IHp (sub_expr_valid _ _ He)).
+      destruct (synth_sub_expr _ H0 He) as [t' [f' [[H3|H3] H4]]];
+        assert (Hf': f2 p = f' []) by
+        (specialize (H4 []); rewrite app_nil_r in H4; assumption);
+        rewrite H4 in H2; destruct e'.
+      + inv Hf.
+      + _gen_eq_spec_ts; inv Hf; inv H3; simpl in Hf'; apply IHp in Hf';
+        simpl in H2; subst.
+        * apply synth_root in H8. congruence.
+        * apply check_root in H8. congruence.
+        * apply check_root in H11. congruence.
+        * apply synth_root in H11. congruence.
+      + _gen_eq_spec_ts. inv Hf. rewrite He. apply IHp. inv H3. simpl in *.
+        apply synth_root in H1. congruence.
+      + _gen_eq_spec_ts. inv Hf. rewrite He. inv H3. simpl in *.
+        destruct (synth_must_be_determine H1). congruence.
+      + _gen_eq_spec_ts. inv Hf; inv H3.
+        * rewrite (max_l _ _ (synth_check_determine_order H8 H11 (le_refl _))) in *.
+          destruct (synth_must_be_determine H8). simpl in *. congruence.
+        * rewrite (max_r _ _ (synth_check_determine_order H11 H8 (le_refl _))) in *.
+          destruct (synth_must_be_determine H11). simpl in *.
+          apply check_root in H8. congruence.
+        * rewrite (max_l _ _ (synth_check_determine_order H8 H11 (le_refl _))) in *.
+          destruct (synth_must_be_determine H8). simpl in *.
+          apply check_root in H11. congruence.
+        * rewrite (max_r _ _ (synth_check_determine_order H11 H8 (le_refl _))) in *.
+          destruct (synth_must_be_determine H11). simpl in *. congruence.
+      + admit.
+      + admit.
+      + admit.
+      + admit.
+      + admit.
+      + admit.
+      + admit.
+      + admit.
+      + inv Hf.
+      + _gen_eq_spec_ts; inv Hf; inv H3; try (inv H5); simpl in Hf'; apply IHp in Hf';
+        simpl in H2; subst.
+        * apply check_root in H8. congruence.
+        * apply check_root in H11. congruence.
+      + _gen_eq_spec_ts. inv Hf. rewrite He. apply IHp. inv H3. inv H.
+        simpl in *. apply check_root in H1. congruence.
+      + _gen_eq_spec_ts. inv Hf. rewrite He. inv H3. inv H1. simpl in *.
+        destruct (synth_must_be_determine H7). simpl in *. congruence.
+      + _gen_eq_spec_ts. inv Hf; inv H3; inv H7.
+        * rewrite (max_l _ _ (synth_check_determine_order H10 H13 (le_refl _))) in *.
+          destruct (synth_must_be_determine H10). simpl in *. congruence.
+        * rewrite (max_r _ _ (synth_check_determine_order H13 H10 (le_refl _))) in *.
+          destruct (synth_must_be_determine H13). simpl in *.
+          apply check_root in H10. congruence.
+        * rewrite (max_l _ _ (synth_check_determine_order H10 H13 (le_refl _))) in *.
+          destruct (synth_must_be_determine H10). simpl in *.
+          apply check_root in H13. congruence.
+        * rewrite (max_r _ _ (synth_check_determine_order H13 H10 (le_refl _))) in *.
+          destruct (synth_must_be_determine H13). simpl in *. congruence.
+      + admit.
+      + admit.
+      + admit.
+      + admit.
+      + admit.
+      + admit.
+      + admit.
+      + admit.
+  Admitted.
+End Equiv.
+
