Rocq/src/TypeSystem.v
@@ -1,0 +1,634 @@
+From Stdlib Require Import Lists.List.
+From Stdlib Require Import PeanoNat.
+From Stdlib Require Import Arith.Compare_dec.
+From Stdlib Require Import Logic.Decidable.
+From Stdlib Require Export Lia.
+
+From Verilog Require Import Expr.
+From Verilog Require Import Path.
+From Verilog Require Import Spec.
+From Verilog Require Import Utils.
+
+Import ListNotations.
+Import Nat.
+
+Import Expr.
+Import Path.
+Import Spec.
+Import Utils.
+
+Set Implicit Arguments.
+
+Module TypeSystem.
+
+  Inductive Resizable : Expr -> Type :=
+  | ResAtom : forall op, Resizable (EAtom op)
+  | ResCast : forall e, Resizable (ECast e)
+  | ResComp : forall lhs rhs, Resizable (EComp lhs rhs)
+  | ResLogic : forall lhs rhs, Resizable (ELogic lhs rhs)
+  | ResRed : forall e, Resizable (EReduction e)
+  | ResAssign : forall lval arg, Resizable (EAssign lval arg)
+  | ResShiftAssign : forall lval arg, Resizable (EShiftAssign lval arg)
+  | ResConcat : forall args, Resizable (EConcat args)
+  | ResRepl : forall amount arg, Resizable (ERepl amount arg)
+  .
+
+  Definition Initial t : path -> option nat :=
+    fun p =>
+      match p with
+      | [] => Some t
+      | _ :: _ => None
+      end
+  .
+
+  Definition ReplaceRoot t (f: path -> option nat) : path -> option nat :=
+    fun p =>
+      match p with
+      | [] => Some t
+      | _ :: _ => f p
+      end
+  .
+
+  Definition Binary t (f g: path -> option nat) : path -> option nat :=
+    fun p =>
+      match p with
+      | [] => Some t
+      | Left :: p => f p
+      | Right :: p => g p
+      | _ :: _ => None
+      end
+  .
+
+  Definition Unary t (f: path -> option nat) : path -> option nat :=
+    fun p =>
+      match p with
+      | [] => Some t
+      | Arg :: p => f p
+      | _ :: _ => None
+      end
+  .
+
+  Definition Ternary t (f g h: path -> option nat) : path -> option nat :=
+    fun p =>
+      match p with
+      | [] => Some t
+      | Arg :: p => f p
+      | Left :: p => g p
+      | Right :: p => h p
+      | _ :: _ => None
+      end
+  .
+
+  Definition Narry t (f_k: list (path -> option nat)) : path -> option nat :=
+    fun p => match p with
+          | [] => Some t
+          | Args i :: p => match nth_error f_k i with
+                         | Some f => f p
+                         | None => None
+                         end
+          | _ :: _ => None
+          end
+  .
+
+  Reserved Notation "e '==>' t '-|' f" (at level 70).
+  Reserved Notation "e '<==' t '-|' f" (at level 70).
+
+  Inductive synth : Expr -> nat -> (path -> option nat) -> Prop :=
+  | AtomS : forall op, EAtom op ==> op -| Initial op
+
+  | LBinOpS : forall a b t fa fb,
+      a ==> t -| fa ->
+      b <== t -| fb ->
+      EBinOp a b ==> t -| Binary t fa fb
+
+  | RBinOpS : forall a b t fa fb,
+      a <== t -| fa ->
+      b ==> t -| fb ->
+      EBinOp a b ==> t -| Binary t fa fb
+
+  | UnOpS : forall e t f,
+      e ==> t -| f ->
+      EUnOp e ==> t -| Unary t f
+
+  | CastS : forall e t f,
+      e ==> t -| f ->
+      ECast e ==> t -| Unary t f
+
+  | LCompS : forall a b t fa fb,
+      a ==> t -| fa ->
+      b <== t -| fb ->
+      EComp a b ==> 1 -| Binary 1 fa fb
+
+  | RCompS : forall a b t fa fb,
+      a <== t -| fa ->
+      b ==> t -| fb ->
+      EComp a b ==> 1 -| Binary 1 fa fb
+
+  | LogicS : forall a b ta tb fa fb,
+      a ==> ta -| fa ->
+      b ==> tb -| fb ->
+      ELogic a b ==> 1 -| Binary 1 fa fb
+
+  | RedS : forall e t f,
+      e ==> t -| f ->
+      EReduction e ==> 1 -| Unary 1 f
+
+  | ShiftS : forall a b t tb fa fb,
+      a ==> t -| fa ->
+      b ==> tb -| fb ->
+      EShift a b ==> t -| Binary t fa fb
+
+  | LAssignS : forall lval e f,
+      e <== lval -| f ->
+      EAssign lval e ==> lval -| Unary lval f
+
+  | RAssignS : forall lval e te f,
+      e ==> te -| f ->
+      lval < te ->
+      EAssign lval e ==> lval -| Unary lval f
+
+  | ShiftAssignS : forall lval e te f,
+      e ==> te -| f ->
+      EShiftAssign lval e ==> lval -| Unary lval f
+
+  | LCondS : forall e a b t te fe fa fb,
+      e ==> te -| fe ->
+      a ==> t -| fa ->
+      b <== t -| fb ->
+      ECond e a b ==> t -| Ternary t fe fa fb
+
+  | RCondS : forall e a b t te fe fa fb,
+      e ==> te -| fe ->
+      a <== t -| fa ->
+      b ==> t -| fb ->
+      ECond e a b ==> t -| Ternary t fe fa fb
+
+  | ConcatS : forall args ts t fs,
+      length args = length ts ->
+      length args = length fs ->
+      (forall n e te fe, nth_error args n = Some e ->
+                    nth_error ts n = Some te ->
+                    nth_error fs n = Some fe ->
+                    e ==> te -| fe) ->
+      t = sum ts ->
+      EConcat args ==> t -| Narry t fs
+
+  | ReplS : forall i e te t f,
+      e ==> te -| f ->
+      t = i * te ->
+      ERepl i e ==> t -| Unary t f
+
+  where "e '==>' n '-|' f" := (synth e n f)
+
+  with check : Expr -> nat -> (path -> option nat) -> Prop :=
+  | ResizeC : forall e s t f,
+      Resizable e ->
+      e ==> s -| f ->
+      s <= t ->
+      e <== t -| ReplaceRoot t f
+
+  | BinOpC : forall a b t fa fb,
+      a <== t -| fa ->
+      b <== t -| fb ->
+      EBinOp a b <== t -| Binary t fa fb
+
+  | UnOpC : forall e t f,
+      e <== t -| f ->
+      EUnOp e <== t -| Unary t f
+
+  | ShiftC : forall a b t tb fa fb,
+      a <== t -| fa ->
+      b ==> tb -| fb ->
+      EShift a b <== t -| Binary t fa fb
+
+  | CondC : forall e a b t te fe fa fb,
+      e ==> te -| fe ->
+      a <== t -| fa ->
+      b <== t -| fb ->
+      ECond e a b <== t -| Ternary t fe fa fb
+
+  where "e '<==' n '-|' f" := (check e n f)
+  .
+
+
+  Lemma synth_root : forall e t f, e ==> t -| f -> f [] = Some t.
+  Proof.
+    intros. inv H; reflexivity.
+  Qed.
+
+  Lemma check_root : forall e t f, e <== t -| f -> f [] = Some t.
+  Proof.
+    intros. inv H; reflexivity.
+  Qed.
+
+  Lemma concat_synth_inj_t: forall args f1 f2 t1 t2,
+      (forall n e, nth_error args n = Some e -> forall t1 t2 f1 f2,
+            e ==> t1 -| f1 -> e ==> t2 -| f2 -> t1 = t2) ->
+      EConcat args ==> t1 -| f1 -> EConcat args ==> t2 -| f2 -> t1 = t2.
+  Proof.
+    intros ? ? ? ? ? He H H0. inv H. inv H0.
+    assert (Heqt: forall n t1 t2,
+               nth_error ts n = Some t1 -> nth_error ts0 n = Some t2 -> t1 = t2).
+    - intros. repeat gen_nth. destruct (He _ _ H7 t1 t2 x1 x0); firstorder.
+    - assert (Heql: ts = ts0). apply nth_ext with (d := 0) (d' := 0).
+      rewrite H2 in *. assumption. intros. apply Heqt with (n := n).
+      apply (nth_error_nth' _ _ H). rewrite <- H2 in H. rewrite H1 in H.
+      apply (nth_error_nth' _ _ H). subst. reflexivity.
+  Qed.
+
+  Lemma concat_synth_inj_f: forall args t1 t2 f1 f2,
+      (forall n e, nth_error args n = Some e -> forall t1 t2 f1 f2,
+            e ==> t1 -| f1 -> e ==> t2 -| f2 -> t1 = t2 /\ forall p, f1 p = f2 p) ->
+      EConcat args ==> t1 -| f1 -> EConcat args ==> t2 -| f2 -> forall p, f1 p = f2 p.
+  Proof.
+    intros ? ? ? ? ? He H H0. assert (Heq: t1 = t2).
+    { eapply concat_synth_inj_t. intros. edestruct He.
+      apply H1. apply H2. apply H3. assumption. eassumption. eassumption.
+    } subst.
+    inv H. inv H0. intros.
+    assert (Heqf: forall n f1 f2, nth_error fs n = Some f1 -> nth_error fs0 n = Some f2 ->
+                             forall p, f1 p = f2 p).
+    { intros. repeat gen_nth. destruct (He _ _ H8 x2 x0 f1 f2); firstorder. }
+    destruct p as [|[]]; try reflexivity. simpl. destruct (nth_error fs i) eqn:Hfs.
+    - repeat gen_nth. rewrite H0. apply Heqf with (n := i); assumption.
+    - destruct (nth_error fs0 i) eqn:Hfs0; try reflexivity. exfalso. repeat gen_nth.
+      rewrite H1 in Hfs. discriminate Hfs.
+  Qed.
+
+  Lemma concat_synth_order_f: forall args t1 t2 f1 f2,
+      (forall n e, nth_error args n = Some e -> forall t1 t2 f1 f2,
+            e ==> t1 -| f1 -> e ==> t2 -| f2 ->
+            t1 = t2 /\ forall p, le_option_nat (f1 p) (f2 p)) ->
+      EConcat args ==> t1 -| f1 -> EConcat args ==> t2 -| f2 ->
+      forall p, le_option_nat (f1 p) (f2 p).
+  Proof.
+    intros ? ? ? ? ? He H H0. assert (Heq: t1 = t2).
+    { eapply concat_synth_inj_t. intros. edestruct He.
+      apply H1. apply H2. apply H3. assumption. eassumption. eassumption.
+    } subst.
+    inv H. inv H0. intros.
+    assert (Hltf: forall n f1 f2, nth_error fs n = Some f1 -> nth_error fs0 n = Some f2 ->
+                             forall p, le_option_nat (f1 p) (f2 p)).
+    { intros. repeat gen_nth. destruct (He _ _ H8 x2 x0 f1 f2); firstorder. }
+    destruct p as [|[]]; try reflexivity. simpl. destruct (nth_error fs i) eqn:Hfs.
+    - repeat gen_nth. rewrite H0. apply Hltf with (n := i); assumption.
+    - destruct (nth_error fs0 i) eqn:Hfs0; try reflexivity.
+  Qed.
+
+  Theorem check_can_grow : forall e t f, e <== t -| f -> forall s, t <= s -> exists f', e <== s -| f'.
+  Proof.
+    Ltac _check_can_grow_tac :=
+      match goal with
+      | [ HRes: Resizable _, H: _ ==> ?x -| _, Hle: ?x <= ?y |- ?e <== ?z -| _ ] =>
+          apply (ResizeC HRes H); apply (le_trans x y z); assumption
+      | [ H: _ <== _ -| _ |- ex _ ] => inv H; eexists; _check_can_grow_tac
+      end
+    .
+    induction e using Expr_ind; intros; try _check_can_grow_tac.
+    - inv H. inv H1. edestruct IHe1; edestruct IHe2; try eassumption.
+      eexists. constructor; eassumption.
+    - inv H. inv H1. edestruct IHe; try eassumption. eexists. constructor. eassumption.
+    - inv H. inv H1. edestruct IHe1; try eassumption. eexists. apply (ShiftC H H6).
+    - inv H. inv H1. edestruct IHe2; edestruct IHe3; try eassumption.
+      eexists. eapply (CondC H4); eassumption.
+  Qed.
+
+  Lemma check_grow_synth_and_synth_inj :
+    forall e, (forall t s f1 f2, e ==> t -| f1 -> e <== s -| f2 -> t <= s) /\
+           (forall t1 t2 f1 f2, e ==> t1 -| f1 -> e ==> t2 -| f2 -> t1 = t2) /\
+           (forall t f1 f2, e ==> t -| f1 -> e ==> t -| f2 -> forall p, f1 p = f2 p) /\
+           (forall t f1 f2, e <== t -| f1 -> e <== t -| f2 -> forall p, f1 p = f2 p) /\
+           (forall t f1 f2, e ==> t -| f1 -> e <== t -| f2 -> forall p, f1 p = f2 p) /\
+           (forall t s f1 f2, e ==> t -| f1 -> e <== s -| f2 -> forall p, le_option_nat (f1 p) (f2 p)) /\
+           (forall t s f1 f2, e <== t -| f1 -> e <== s -| f2 -> t <= s ->
+                         forall p, le_option_nat (f1 p) (f2 p)).
+  Proof.
+    Ltac _invHyp_inj :=
+      match goal with
+      | [ H: _ _ ==> _ -| _ |- _ ] => inv H; try _invHyp_inj
+      | [ H: _ _ <== _ -| _ |- _ ] => inv H; try _invHyp_inj
+      | [ H: Resizable _ |- _ ] => inv H
+      end
+    .
+    Ltac _eq_gen_inj :=
+      match goal with
+      | [ A: ?e ==> ?t -| _, B: ?e ==> ?s -| _, H: forall _ _ _ _, _ -> _ -> _ = _ |- _ ] =>
+          let Heq := fresh in assert (Heq: t = s) by apply (H _ _ _ _ A B);
+                              clear H; subst
+      | [ A: ?e ==> ?t -| _, B: ?e <== ?s -| _, H: forall _ _ _ _, _ -> _ -> _ <= _ |- _ ] =>
+          let Hlt := fresh in assert (Hlt: t <= s) by apply (H _ _ _ _ A B);
+                              clear H; try _eq_gen_inj; try lia
+      | [ H: ?a <= ?b, P: ?b <= ?a |- _ ] =>
+          let Heq := fresh in assert (Heq: a = b) by apply (le_antisymm _ _ H P);
+                              clear H; clear P; subst
+      end
+    .
+    Ltac _tac_inj :=
+      match goal with
+      (* Values *)
+      | [ |- _ = _ ] => _eq_gen_inj; auto
+      | [  A: ?e ==> ?t -| _, B: ?e <== ?s -| _, H: forall _ _ _ _, _ -> _ -> _ <= _ |- ?t <= ?s ] =>
+          apply (H _ _ _ _ A B)
+      | [ A: ?e ==> ?t -| _, B: ?e ==> ?s -| _, H: forall _ _ _ _, _ -> _ -> _ = _ |- _ ] =>
+          let Heq := fresh in assert (Heq: t = s) by apply (H _ _ _ _ A B);
+                              clear H; subst; auto; _tac_inj
+      (* Functions *)
+      (* - Synth & Check *)
+      | [  A: ?e ==> ?t -| _, B: ?e <== ?t -| _,
+              H: forall _ _ _, _ -> _ -> forall _, _ =  _ |- _ _ = _ _ ] =>
+          apply (H _ _ _ A B) || symmetry; apply (H _ _ _ A B)
+      (* Both synth *)
+      | [ A: ?e ==> ?t -| _, B: ?e ==> ?t -| _,
+              H: forall _ _ _, _ -> _ -> forall _,  _ = _ |- _ _ = _ _ ] =>
+          try _eq_gen_inj; apply (H _ _ _ A B)
+        (* Both check *)
+      | [ A: ?e <== ?t -| ?f1, B: ?e <== ?t -| ?f2,
+              H: forall _ _ _, _ -> _ -> forall _, _ = _ |- ?f1 _ = ?f2 _ ] =>
+          apply (H _ _ _ A B)
+      | [ A: ?e ==> _ -| _, B: ?e <== _ -| _,
+              H: forall _ _ _ _, _ -> _ -> forall _, le_option_nat _ _
+                                         |- le_option_nat _ _ ] =>
+          apply (H _ _ _ _ A B)
+      | [ A: ?e <== ?t -| _, B: ?e <== ?s -| _, C: ?t <= ?s,
+                H: forall _ _ _ _, _ -> _ -> _ -> forall _, le_option_nat _ _
+                                               |- le_option_nat _ _ ] =>
+          apply (H _ _ _ _ A B C)
+      | [ A: ?e ==> ?t -| _, B: ?e ==> ?t -| _,
+              H: forall _ _ _, _ -> _ -> forall _, _ = _ |- le_option_nat _ _ ] =>
+          rewrite (H _ _ _ A B); reflexivity
+      | [ A: ?e <== ?t -| _, B: ?e <== ?t -| _,
+              H: forall _ _ _, _ -> _ -> forall _, _ = _ |- le_option_nat _ _ ] =>
+          rewrite (H _ _ _ A B); reflexivity
+      | [ A: ?e ==> ?t -| _, B: ?e <== ?t -| _,
+              H: forall _ _ _, _ -> _ -> forall _, _ = _ |- le_option_nat _ _ ] =>
+          rewrite (H _ _ _ A B); reflexivity
+      end
+    .
+    induction e using Expr_ind; repeat splitAnd; intros; repeat splitHyp;
+      try (destruct p as [|[]]);
+      try (_invHyp_inj; auto; repeat _tac_inj + _invHyp_inj;
+           simpl; try reflexivity; repeat _tac_inj + _invHyp_inj;
+           simpl; repeat _eq_gen_inj; auto; _tac_inj).
+    - inv H1. assert (Heq: t0 = s0).
+      { eapply (concat_synth_inj_t _ H0 H3). Unshelve.
+        intros. destruct (H _ _ H1). repeat splitHyp. apply (H8 _ _ _ _ H5 H6).
+      } subst. assumption.
+    - eapply (concat_synth_inj_t _ H1 H2). Unshelve.
+      intros. destruct (H _ _ H3). repeat splitHyp. apply (H7 _ _ _ _ H4 H5).
+    - eapply (concat_synth_inj_f _ H2 H3). Unshelve.
+      intros. destruct (H _ _ H4). repeat splitHyp. splitAnd. apply (H8 _ _ _ _ H5 H6).
+      intros. subst. apply (H9 _ _ _ H5 H6).
+    - inv H3. inv H4. assert (Heq: forall p, f p = f0 p).
+      { eapply (concat_synth_inj_f _ H6 H8). Unshelve.
+        intros. destruct (H _ _ H4). repeat splitHyp. splitAnd.
+        apply (H13 _ _ _ _ H10 H11). intros. subst. apply (H14 _ _ _ H10 H11).
+      } simpl. apply Heq.
+    - inv H5. assert (Heq: forall p, f1 p = f p).
+      { eapply (concat_synth_inj_f _ H4 H7). Unshelve.
+        intros. destruct (H _ _ H5). repeat splitHyp. splitAnd.
+        apply (H12 _ _ _ _ H9 H10). intros. subst. apply (H13 _ _ _ H9 H10).
+      } simpl. apply Heq.
+    - inv H6. _eq_gen_inj. simpl. rewrite (synth_root H5). trivial.
+    - inv H6. _eq_gen_inj. simpl. eapply (concat_synth_order_f _ H5 H8).
+      Unshelve. intros. destruct (H _ _ H1). repeat splitHyp. repeat splitAnd.
+      apply (H12 _ _ _ _ H6 H10). subst. rewrite (H13 _ _ _ H6 H10). reflexivity.
+    - inv H6. inv H7. _eq_gen_inj. simpl. eapply (concat_synth_order_f _ H10 H12).
+      Unshelve. intros. destruct (H _ _ H1).
+      repeat splitHyp. repeat splitAnd. apply (H16 _ _ _ _ H7 H14). subst.
+      rewrite (H17 _ _ _ H7 H14). reflexivity.
+  Qed.
+
+
+  Theorem synth_check_order : forall e t s f1 f2, e ==> t -| f1 -> e <== s -| f2 -> t <= s.
+  Proof.
+    intros. destruct (check_grow_synth_and_synth_inj e). apply (H1 _ _ _ _ H H0).
+  Qed.
+
+  Theorem synth_inj : forall e t1 t2 f1 f2, e ==> t1 -| f1 -> e ==> t2 -| f2 -> t1 = t2.
+  Proof.
+    intros. destruct (check_grow_synth_and_synth_inj e).
+    repeat splitHyp. apply (H2 _ _ _ _ H H0).
+  Qed.
+
+  Theorem synth_inj_f : forall e t1 t2 f1 f2, e ==> t1 -| f1 -> e ==> t2 -| f2 -> forall p, f1 p = f2 p.
+  Proof.
+    intros. destruct (check_grow_synth_and_synth_inj e).
+    repeat splitHyp. rewrite (H2 _ _ _ _ H H0) in H. apply (H3 _ _ _ H H0).
+  Qed.
+
+  Theorem synth_check_inj_f : forall e t f1 f2, e ==> t -| f1 -> e <== t -| f2 -> forall p, f1 p = f2 p.
+  Proof.
+    intros. destruct (check_grow_synth_and_synth_inj e). firstorder.
+  Qed.
+
+  Theorem check_inj_f : forall e t f1 f2, e <== t -| f1 -> e <== t -| f2 -> forall p, f1 p = f2 p.
+  Proof.
+    intros. destruct (check_grow_synth_and_synth_inj e). firstorder.
+  Qed.
+
+  Theorem synth_check_order_f : forall e t s f1 f2,
+      e ==> t -| f1 -> e <== s -| f2 -> forall p n1 n2, f1 p = Some n1 -> f2 p = Some n2 -> n1 <= n2.
+  Proof.
+    intros. destruct (check_grow_synth_and_synth_inj e). unfold le_option_nat in *.
+    repeat splitHyp. apply (H8 _ _ _ _ H) with (p := p) in H0. rewrite H1 in H0.
+    rewrite H2 in H0. assumption.
+  Qed.
+
+  Theorem check_order_f : forall e t s f1 f2,
+      e <== t -| f1 -> e <== s -| f2 -> t <= s ->
+      forall p n1 n2, f1 p = Some n1 -> f2 p = Some n2 -> n1 <= n2.
+  Proof.
+    intros. destruct (check_grow_synth_and_synth_inj e). unfold le_option_nat in *.
+    repeat splitHyp. apply (H10 _ _ _ _ H H0) with (p := p) in H1. rewrite H2 in H1.
+    rewrite H3 in H1. assumption.
+  Qed.
+
+  Lemma synth_can_check : forall e t s f, e ==> t -| f -> t <= s -> exists g, e <== s -| g.
+  Proof.
+    induction e using Expr_ind; intros; try (eexists; apply ResizeC with (s := t0);
+                                             [constructor | eassumption | assumption]).
+    - inv H.
+      + destruct (IHe1 _ _ _ H3 H0). destruct (check_can_grow H6 H0).
+        eexists. apply BinOpC; eassumption.
+      + destruct (IHe2 _ _ _ H6 H0). destruct (check_can_grow H3 H0).
+        eexists. apply BinOpC; eassumption.
+    - inv H. destruct (IHe _ _ _ H2 H0). eexists. constructor. eassumption.
+    - inv H. destruct (IHe1 _ _ _ H3 H0). eexists. apply (ShiftC H H6).
+    - inv H.
+      + destruct (IHe2 _ _ _ H7 H0). destruct (check_can_grow H8 H0).
+        eexists. apply (CondC H4 H H1).
+      + destruct (IHe3 _ _ _ H8 H0). destruct (check_can_grow H7 H0).
+        eexists. apply (CondC H4 H1 H).
+  Qed.
+
+  Theorem synth_check : forall e t f, e ==> t -| f -> forall s, t <= s <-> exists g, e <== s -| g.
+  Proof.
+    split; intros.
+    - apply (synth_can_check H H0).
+    - destruct H0. apply (synth_check_order H H0).
+  Qed.
+
+  Theorem synth_determine : forall e, exists f, e ==> determine e -| f.
+  Proof.
+    induction e using Expr_ind; repeat existsHyp.
+    - eexists. constructor.
+    - destruct (max_dec_bis (determine e1) (determine e2)) as [[H1 H2]|[H1 H2]].
+      + destruct (synth_can_check H H2). eexists. simpl. rewrite H1.
+        constructor; eassumption.
+      + destruct (synth_can_check H0 H2). eexists. simpl. rewrite H1.
+        constructor; eassumption.
+    - eexists. constructor. eassumption.
+    - eexists. constructor. eassumption.
+    - destruct (max_dec_bis (determine e1) (determine e2)) as [[H1 H2]|[H1 H2]].
+      + destruct (synth_can_check H H2). eexists. simpl. eapply LCompS; eassumption.
+      + destruct (synth_can_check H0 H2). eexists. simpl. eapply RCompS; eassumption.
+    - eexists. eapply LogicS; eassumption.
+    - eexists. eapply RedS; eassumption.
+    - eexists. eapply ShiftS; eassumption.
+    - destruct (le_gt_dec (determine e) op).
+      + destruct (synth_can_check H l). eexists. eapply LAssignS; eassumption.
+      + eexists. eapply RAssignS; eassumption.
+    - eexists. eapply ShiftAssignS; eassumption.
+    - destruct (max_dec_bis (determine e2) (determine e3)) as [[H2 H3]|[H2 H3]].
+      + destruct (synth_can_check H H3). eexists. simpl. rewrite H2.
+        eapply LCondS; eassumption.
+      + destruct (synth_can_check H0 H3). eexists. simpl. rewrite H2.
+        eapply RCondS; eassumption.
+    - assert (Hfs: exists fs, length fs = length args /\ forall n e t f,
+                   nth_error args n = Some e ->
+                   nth_error (map determine args) n = Some t ->
+                   nth_error fs n = Some f -> e ==> t -| f).
+      + induction args.
+        * eexists []. split. reflexivity. intros []; intros; discriminate H0.
+        * edestruct IHargs. intros. destruct (H (S n) e H0). exists x. assumption.
+          destruct H0. destruct (H 0 a). reflexivity. exists (x0 :: x). split.
+          -- simpl. rewrite H0. reflexivity.
+          -- intros. destruct n. inv H3. inv H4. inv H5. assumption.
+             simpl in *. firstorder.
+      + destruct Hfs as [fs [H1 H2]]. eexists.
+        apply ConcatS with (ts := map determine args).
+        * symmetry. apply length_map.
+        * symmetry. eassumption.
+        * assumption.
+        * reflexivity.
+    - eexists. eapply ReplS. eassumption. reflexivity.
+  Qed.
+
+  Theorem synth_must_be_determine : forall e t f,
+      e ==> t -| f -> t = determine e /\ f [] = Some (determine e).
+  Proof.
+    intros. splitAnd.
+    - destruct (synth_determine e). apply (synth_inj H H0).
+    - rewrite (synth_root H). subst. reflexivity.
+  Qed.
+
+  Definition P e s := forall t, s <= t -> exists g, e <== t -| g.
+
+  Theorem synth_minimal_check : forall e s, P e s -> (forall u, P e u -> s <= u) -> exists f, e ==> s -| f.
+  Proof.
+    unfold P. intros. destruct synth_determine with (e := e) as [x Hx].
+    assert (Heq: s = determine e).
+    { apply le_antisymm.
+      - apply H0. intros. apply (synth_can_check Hx H1).
+      - destruct (H s). reflexivity. apply (synth_check_order Hx H1).
+    } subst. exists x. assumption.
+  Qed.
+
+
+  Lemma func_on_path : forall e,
+      (forall t f, e ==> t -| f -> forall p, IsPath e p <-> exists n, f p = Some n) /\
+        (forall t f, e <== t -| f -> forall p, IsPath e p <-> exists n, f p = Some n).
+  Proof.
+    Ltac _invHyp_fun_path :=
+      match goal with
+      | [ H: IsPath (_ _) _ |- _ ] => inv H
+      | [ H: (_ _) ==> _ -| _ |- _ ] => inv H
+      | [ H: (_ _) <== _ -| _ |- _ ] => inv H
+      | [ H: ex _ |- _ ] => inv H
+      end
+    .
+    Ltac _tac_fun_path :=
+      match goal with
+      | [ H1: _ ==> _ -| _, H2: forall _ _, _ ==> _ -| _ -> _  |- _ ] =>
+        try constructor; rewrite (H2 _ _ H1); eexists; eassumption
+      | [ H1: _ <== _ -| _, H2: forall _ _, _ <== _ -| _ -> _  |- _ ] =>
+          try constructor; rewrite (H2 _ _ H1); eexists; eassumption
+      | [ |- IsPath _ [] ] => constructor
+      end
+    .
+    induction e using Expr_ind; repeat split; intros; repeat splitHyp;
+      repeat _invHyp_fun_path; try (try (eexists; reflexivity); firstorder);
+      try (destruct p as [|[]]; simpl in *; discriminate H || inv H; _tac_fun_path).
+    - destruct (H _ _ H3). repeat gen_nth. simpl. rewrite H7.
+      assert (He: e ==> x0 -| x) by apply (H6 _ _ _ _ H3 H5 H7). firstorder.
+    - destruct p as [|[]]; simpl in *; discriminate H0 || inv H0. constructor.
+      destruct (nth_error fs i) eqn:Hnth. repeat gen_nth. apply (P_ConcatArgs _ _ H0).
+      destruct (H _ _ H0). apply (H5 _ _ _ _ H0 H1) in Hnth. _tac_fun_path.
+      discriminate H2.
+    - destruct (H _ _ H3). repeat gen_nth. simpl. rewrite H9.
+      assert (He: e ==> x0 -| x) by apply (H8 _ _ _ _ H3 H7 H9). firstorder.
+    - destruct p as [|[]]; simpl in *; discriminate H0 || inv H0. constructor.
+      destruct (nth_error fs i) eqn:Hnth. repeat gen_nth. apply (P_ConcatArgs _ _ H0).
+      destruct (H _ _ H0). apply (H7 _ _ _ _ H0 H1) in Hnth. _tac_fun_path.
+      discriminate H3.
+  Qed.
+
+
+  Theorem synth_f_path : forall e t f, e ==> t -| f -> forall p, IsPath e p <-> exists n, f p = Some n.
+  Proof.
+    intros e. destruct (func_on_path e). assumption.
+  Qed.
+
+
+  Theorem check_f_path : forall e t f, e <== t -| f -> forall p, IsPath e p <-> exists n, f p = Some n.
+  Proof.
+    intros e. destruct (func_on_path e). assumption.
+  Qed.
+
+  Lemma f_sub_exp : forall e,
+      (forall t f, e ==> t -| f -> forall p e', e @[p] = Some e' ->
+                                  exists t' f', (e' ==> t' -| f' \/ e' <== t' -| f') /\
+                                             forall k, f (p ++ k) = f' k) /\
+        (forall t f, e <== t -| f -> forall p e', e @[p] = Some e' ->
+                                    exists t' f', (e' ==> t' -| f' \/ e' <== t' -| f') /\
+                                               forall k, f (p ++ k) = f' k).
+  Proof.
+    Ltac _inv_se_f :=
+      match goal with
+      | [ H: _ _ @[ _ ] = _ |- _ ] => inv H
+      end
+    .
+    Ltac _inv_ts_f :=
+      match goal with
+      | [ H: _ _ ==> _ -| _ |- _ ] => inv H
+      | [ H: _ _ <== _ -| _ |- _ ] => inv H
+      | [ H: Resizable (_ _) |- _ ] => inv H
+      end
+    .
+    induction e using Expr_ind; split; intros; repeat splitHyp;
+      destruct p as [|[]]; _inv_se_f; try (exists t0; exists f; split; auto; intros; reflexivity);
+      repeat _inv_ts_f; firstorder.
+    - destruct (nth_error args i) eqn:Hnth; try (discriminate H3). destruct (H _ _ Hnth).
+      clear H. repeat _inv_ts_f. repeat gen_nth. simpl. rewrite H.
+      assert (He: e ==> x0 -| x) by apply (H5 _ _ _ _ Hnth H4 H).
+      firstorder.
+    - destruct (nth_error args i) eqn:Hnth; try (discriminate H3). destruct (H _ _ Hnth).
+      clear H. repeat _inv_ts_f. repeat gen_nth. simpl. rewrite H.
+      assert (He: e ==> x0 -| x) by apply (H7 _ _ _ _ Hnth H2 H).
+      firstorder.
+  Qed.
+
+  Theorem synth_sub_expr : forall e t f p e',
+      e ==> t -| f ->  e @[p] = Some e' ->
+      exists t' f', (e' ==> t' -| f' \/ e' <== t' -| f') /\ forall k, f (p ++ k) = f' k.
+  Proof.
+    intros. destruct (f_sub_exp e). firstorder.
+  Qed.
+
+  Theorem check_sub_expr : forall e t f p e',
+      e <== t -| f ->  e @[p] = Some e' ->
+      exists t' f', (e' ==> t' -| f' \/ e' <== t' -| f') /\ forall k, f (p ++ k) = f' k.
+  Proof.
+    intros. destruct (f_sub_exp e). firstorder.
+  Qed.
+End TypeSystem.
