Rocq/scripts/generate_doc.sh
@@ -1,0 +1,3 @@
+#!/bin/bash
+mkdir -p doc
+coqdoc --html -d doc -R _build/default/src Verilog _build/default/src/*.v
